checkpoint: the correctness of SBpass.
1) changed SBpass to make proofs
2) changed returnUpdateLocals, which should return result from callee to
caller even if caller does not need the result. The old design ignored
such return results, which is not true because that means the callee
knows what signature its callsite uses.

We did not find the problem before because the proofs did not need the
fact --- callee and caller may use different signatures, while the
SoftBound proofs does.



git-svn-id: https://webdav.seas.upenn.edu/svn/sol/vol@3009 eef5ea85-cc2e-0410-bd84-0fae1f012da8

src/SoftBound/sb_ds_def.v
@@ -210,26 +210,39 @@ Definition switchToNewBasicBlock (TD:TargetData) (M:mem) (Dest:block)
   returning arbitrary values.
 *)
 
-Definition returnUpdateLocals (TD:TargetData) (M:mem) (c':cmd)
+Definition isReturnPointerTypB t0 : bool :=
+match t0 with
+| typ_function t0 _ _ => isPointerTypB t0
+| _ => false
+end.
+
+Definition returnResult (TD:TargetData) (M:mem) (rt:typ) (Result:value) 
+  (lc:GVMap) (rm:rmetadata) (gl:GVMap) : option (GenericValue * metadata) :=
+  match getOperandValue TD M Result lc gl with
+  | Some gr =>
+      if isPointerTypB rt then
+        match get_reg_metadata TD M gl rm Result with
+        | Some md => Some (gr, md)
+        | None => None
+        end
+      else Some (gr, (mkMD null null))
+  | _ => None
+  end.
+
+Definition returnUpdateLocals (TD:TargetData) (M:mem) (c':cmd) (rt:typ) 
   (Result:value) (lc lc':GVMap) (rm rm':rmetadata) (gl:GVMap) 
   : option (GVMap * rmetadata) :=
-    match c' with
-    | insn_call id0 false _ t _ _ =>
-        match getOperandValue TD M Result lc gl with
-        | Some gr =>
-            match t with
-            | typ_function (typ_pointer _) _ _ =>
-              match get_reg_metadata TD M gl rm Result with
-              | Some md => Some (prop_reg_metadata lc' rm' id0 gr md)
-              | None => Some 
-                  (prop_reg_metadata lc' rm' id0 gr (mkMD null null))
-              end
-            | _ => Some (updateAddAL _ lc' id0 gr, rm')
-            end
-        | _ => None
-        end
-    | _ => Some (lc', rm')
-    end.
+  match returnResult TD M rt Result lc rm gl with
+  | Some (gr,md) =>
+      match c' with
+      | insn_call id0 false _ t _ _ =>
+          if isReturnPointerTypB t then 
+            Some (prop_reg_metadata lc' rm' id0 gr md)
+          else Some (updateAddAL _ lc' id0 gr, rm')
+      | _ => Some (lc', rm')
+      end
+  | _ => None
+  end.
 
 Definition exCallUpdateLocals (ft:typ) (noret:bool) (rid:id) 
   (oResult:option GenericValue) (lc :GVMap) (rm:rmetadata) 
@@ -291,7 +304,8 @@ Inductive dsInsn : State -> State -> trace -> Prop :=
     lc' rm' EC Mem MM Mem' als als' lc'' rm'',   
   Instruction.isCallInst c' = true ->
   free_allocas TD Mem als = Some Mem' ->
-  returnUpdateLocals TD Mem' c' Result lc lc' rm rm' gl = Some (lc'', rm'') ->
+  returnUpdateLocals TD Mem' c' RetTy Result lc lc' rm rm' gl = 
+    Some (lc'', rm'') ->
   dsInsn 
     (mkState S TD Ps 
       ((mkEC F B nil (insn_return rid RetTy Result) lc rm als)::
@@ -676,7 +690,7 @@ Inductive dsInsn : State -> State -> trace -> Prop :=
   LLVMopsem.lookupExFdecViaGV TD Mem Ps gl lc fs fv = 
     Some (fdec_intro (fheader_intro fa rt fid la va)) -> 
   LLVMgv.params2GVs TD Mem lp lc gl = Some gvs ->
-  LLVMopsem.callExternalFunction Mem fid gvs = (oresult, Mem') ->
+  LLVMopsem.callExternalFunction Mem fid gvs = Some (oresult, Mem') ->
   exCallUpdateLocals ft noret rid oresult lc rm = Some (lc',rm') ->
   dsInsn 
     (mkState S TD Ps 
