src/SoftBound/sb_ds_trans_correct.v
@@ -1,0 +1,657 @@
+Add LoadPath "../ssa/ott".
+Add LoadPath "../ssa/monads".
+Add LoadPath "../ssa".
+Add LoadPath "../ssa/compcert".
+Add LoadPath "../../../theory/metatheory_8.3".
+Add LoadPath "../TV".
+Require Import ssa_def.
+Require Import ssa_lib.
+Require Import ssa_dynamic.
+Require Import trace.
+Require Import Memory.
+Require Import genericvalues.
+Require Import alist.
+Require Import Integers.
+Require Import Values.
+Require Import Coqlib.
+Require Import monad.
+Require Import Metatheory.
+Require Import Znumtheory.
+Require Import sb_ds_def.
+Require Import sb_ds_trans.
+
+Import SB_ds_pass.
+
+(* Simulation *)
+
+Definition meminj_no_overlap (f: meminj) (m: mem) : Prop :=
+  forall b1 b1' delta1 b2 b2' delta2,
+  b1 <> b2 ->
+  f b1 = Some (b1', delta1) ->
+  f b2 = Some (b2', delta2) ->
+  b1' <> b2'.
+
+Lemma meminj_no_overlap__implies : forall f m,
+  meminj_no_overlap f m -> Mem.meminj_no_overlap f m.
+Proof.
+  intros f m J.
+  unfold meminj_no_overlap in J.
+  unfold Mem.meminj_no_overlap.
+  eauto.
+Qed.
+
+Record wf_sb_mi maxb mi Mem1 Mem2 := mk_wf_sb_mi {
+  Hno_overlap : meminj_no_overlap mi Mem1;
+  Hnull : mi Mem.nullptr = Some (Mem.nullptr, 0);
+  Hmap1 : forall b, b >= Mem.nextblock Mem1 -> mi b = None;
+  Hmap2 : forall b1 b2 delta2, 
+    mi b1 = Some (b2, delta2) -> b2 < Mem.nextblock Mem2;
+  mi_freeblocks: forall b, ~(Mem.valid_block Mem1 b) -> mi b = None;
+  mi_mappedblocks: forall b b' delta, 
+    mi b = Some(b', delta) -> Mem.valid_block Mem2 b';
+  mi_range_block: forall b b' delta, 
+    mi b = Some(b', delta) -> delta = 0;
+  mi_bounds: forall b b' delta, 
+    mi b = Some(b', delta) -> Mem.bounds Mem1 b = Mem.bounds Mem2 b';
+  mi_globals : forall b, b <= maxb -> mi b = Some (b, 0)
+  }.
+
+Definition gv_inject (mi: Values.meminj) (gv gv':GenericValue) : Prop :=
+let '(vals,mks) := List.split gv in 
+let '(vals',mks') := List.split gv' in 
+val_list_inject mi vals vals' /\ mks = mks'.
+
+Definition reg_simulation (mi:Values.meminj) TD gl (rm1:SBopsem.rmetadata) 
+  (rm2:rmap) Mem1 Mem2 (lc1 lc2:GVMap) : Prop :=
+(forall i0 gv1, 
+  lookupAL _ lc1 i0 = Some gv1 -> 
+  exists gv2, 
+    lookupAL _ lc2 i0 = Some gv2 /\ gv_inject mi gv1 gv2
+) /\
+(forall vp bgv1 egv1, 
+  SBopsem.get_reg_metadata TD Mem1 gl rm1 vp = 
+    Some (SBopsem.mkMD bgv1 egv1) -> 
+  exists bv2, exists ev2, exists bgv2, exists egv2,
+    get_reg_metadata rm2 vp = Some (bv2, ev2) /\
+    getOperandValue TD Mem2 bv2 lc2 gl = Some bgv2 /\
+    getOperandValue TD Mem2 ev2 lc2 gl = Some egv2 /\
+    gv_inject mi bgv1 bgv2 /\
+    gv_inject mi egv1 egv2
+).
+
+Fixpoint wf_global (maxb:Values.block) (gv:GenericValue) 
+  : Prop :=
+match gv with
+| nil => True
+| (Vptr b _,_)::gv' => b <= maxb /\ wf_global maxb gv'
+| _::gv' => wf_global maxb gv'
+end.
+
+Fixpoint wf_globals maxb (gl:GVMap) : Prop :=
+match gl with
+| nil => True
+| (_,gv)::gl' => wf_global maxb gv /\ wf_globals maxb gl'
+end.
+
+Definition mem_simulation (mi:Values.meminj) TD (max_gblock:Values.block) 
+  (MM1:SBopsem.mmetadata) (Mem1 Mem2:mem) : Prop :=
+Mem.mem_inj mi Mem1 Mem2 /\
+0 <= max_gblock < Mem.nextblock Mem2 /\
+(forall lc2 gl b ofs bgv egv als addrb addre bid0 eid0 pgv' fs F B cs tmn S Ps 
+    EC v,  
+  wf_globals max_gblock gl -> 
+  SBopsem.get_mem_metadata TD MM1 (ptr2GV TD (Vptr b ofs)) = 
+    SBopsem.mkMD bgv egv -> 
+  gv_inject mi (ptr2GV TD (Vptr b ofs)) pgv' ->
+  getOperandValue TD Mem2 v lc2 gl = Some pgv' ->
+  exists bgv', exists egv',
+  LLVMopsem.dsInsn 
+    (LLVMopsem.mkState S TD Ps 
+      ((LLVMopsem.mkEC F B 
+        (insn_call fake_id true attrs gmd_typ gmd_fn
+           ((p8,v)::
+            (p8,(value_id addrb))::
+            (p8,(value_id addre))::nil)::
+         insn_load bid0 p8 (value_id addrb) Align.Zero::
+         insn_load eid0 p8 (value_id addre) Align.Zero::   
+         cs) 
+        tmn lc2 als)
+        ::EC) gl fs Mem2)
+    (LLVMopsem.mkState S TD Ps 
+       ((LLVMopsem.mkEC F B cs tmn 
+         (updateAddAL _ (updateAddAL _ lc2 bid0 bgv') eid0 egv') als)::EC) 
+        gl fs Mem2)
+    trace_nil /\
+    gv_inject mi bgv bgv' /\
+    gv_inject mi egv egv'
+).
+
+Definition alloca_simulation (mi:Values.meminj) (b1 b2:Values.block) : Prop := 
+  mi b1 = Some(b2, 0).
+
+Fixpoint allocas_simulation_suffix (mi:Values.meminj) 
+  (als1 als2:list Values.block) : Prop := 
+match als1, als2 with
+| nil, nil => True
+| b1::als1', b2::als2' => alloca_simulation mi b1 b2 /\
+    allocas_simulation_suffix mi als1' als2'
+| _, _ => False
+end.
+
+Definition allocas_simulation TD (mi:Values.meminj) lc2 addrb addre 
+  (als1 als2:list mblock) : Prop := 
+let als1' := rev als1 in
+let als2' := rev als2 in
+match als2' with
+| baddrb::baddre::als2'' => allocas_simulation_suffix mi als1 als2 /\
+    lookupAL _ lc2 addrb = Some (ptr2GV TD (Vptr baddrb (Int.zero 31))) /\
+    lookupAL _ lc2 addre = Some (ptr2GV TD (Vptr baddre (Int.zero 31))) /\
+    forall b1 b2 d, mi b1 = Some (b2, d) -> b2 <> baddrb /\ b2 <> baddre
+| _ => False
+end.
+
+Definition sbEC_simulates_EC_tail (TD:TargetData) M1 M2 gl (mi:Values.meminj) 
+  (sbEC:SBopsem.ExecutionContext) (EC:LLVMopsem.ExecutionContext) : Prop :=
+  match (sbEC, EC) with
+  | (SBopsem.mkEC f1 b1 ((insn_call i0 nr ca t0 v p)::cs13) tmn1 lc1 rm1 als1, 
+     LLVMopsem.mkEC f2 b2 cs2 tmn2 lc2 als2) =>
+       let '(fdef_intro fh1 bs1) := f1 in
+       let '(fdef_intro fh2 bs2) := f2 in
+       let '(los, nts) := TD in
+       trans_fdef nts f1 = Some f2 /\
+       tmn1 = tmn2 /\
+       (exists n, nth_error bs1 n = Some b1 /\ nth_error bs2 n = Some b2) /\
+       (exists l1, exists ps1, exists cs11, 
+         b1 = block_intro l1 ps1 (cs11++(insn_call i0 nr ca t0 v p)::cs13) tmn1)
+         /\
+       (exists l2, exists ps2, exists cs21,
+         b2 = block_intro l2 ps2 (cs21++cs2) tmn2) /\
+       exists ex_ids, exists rm2, 
+       exists addrb, exists ex_ids1, exists addre, exists ex_ids2, 
+       exists ex_ids3, exists ex_ids4, exists cs22, exists cs23, exists cs24,
+         gen_metadata_fdef nts (getFdefLocs f1) nil f1 = Some (ex_ids, rm2) /\
+         reg_simulation mi TD gl rm1 rm2 M1 M2 lc1 lc2 /\
+         (addrb,ex_ids1) = mk_tmp ex_ids /\
+         (addre,ex_ids2) = mk_tmp ex_ids1 /\
+         allocas_simulation TD mi lc2 addrb addre als1 als2 /\
+         incl ex_ids2 ex_ids3 /\ 
+         call_suffix i0 nr ca t0 v p rm2 = Some cs22 /\
+         trans_cmds ex_ids1 addrb addre rm2 cs13 = Some (ex_ids4,cs23) /\
+         trans_terminator rm2 tmn1 = Some cs24 /\
+         cs2 = cs22 ++ cs23 ++ cs24
+  | _ => False
+  end.
+
+Definition sbEC_simulates_EC_head (TD:TargetData) M1 M2 gl (mi:Values.meminj) 
+  (sbEC:SBopsem.ExecutionContext) (EC:LLVMopsem.ExecutionContext) : Prop :=
+  match (sbEC, EC) with
+  | (SBopsem.mkEC f1 b1 cs12 tmn1 lc1 rm1 als1, 
+     LLVMopsem.mkEC f2 b2 cs2 tmn2 lc2 als2) =>
+       let '(fdef_intro fh1 bs1) := f1 in
+       let '(fdef_intro fh2 bs2) := f2 in
+       let '(los, nts) := TD in
+       trans_fdef nts f1 = Some f2 /\
+       tmn1 = tmn2 /\
+       (exists n, nth_error bs1 n = Some b1 /\ nth_error bs2 n = Some b2) /\
+       (exists l1, exists ps1, exists cs11, 
+         b1 = block_intro l1 ps1 (cs11++cs12) tmn1) /\
+       (exists l2, exists ps2, exists cs21,
+         b2 = block_intro l2 ps2 (cs21++cs2) tmn2) /\
+       exists ex_ids, exists rm2, 
+       exists addrb, exists ex_ids1, exists addre, exists ex_ids2, 
+       exists ex_ids3, exists ex_ids4, exists cs22, exists cs23,
+         gen_metadata_fdef nts (getFdefLocs f1) nil f1 = Some (ex_ids, rm2) /\
+         reg_simulation mi TD gl rm1 rm2 M1 M2 lc1 lc2 /\
+         (addrb,ex_ids1) = mk_tmp ex_ids /\
+         (addre,ex_ids2) = mk_tmp ex_ids1 /\
+         allocas_simulation TD mi lc2 addrb addre als1 als2 /\
+         incl ex_ids2 ex_ids3 /\ 
+         trans_cmds ex_ids1 addrb addre rm2 cs12 = Some (ex_ids4,cs22) /\
+         trans_terminator rm2 tmn1 = Some cs23 /\
+         cs2 = cs22 ++ cs23
+  end.
+
+Fixpoint sbECs_simulate_ECs_tail (TD:TargetData) M1 M2 gl (mi:Values.meminj) 
+  (sbECs:SBopsem.ECStack) (ECs:LLVMopsem.ECStack) : Prop :=
+  match sbECs, ECs with
+  | nil, nil => True
+  | sbEC::sbECs', EC::ECs' => 
+      sbEC_simulates_EC_tail TD M1 M2 gl mi sbEC EC /\ 
+      sbECs_simulate_ECs_tail TD M1 M2 gl mi sbECs' ECs'
+  | _, _ => False
+  end.
+
+Definition sbECs_simulate_ECs (TD:TargetData) M1 M2 gl (mi:Values.meminj) 
+  (sbECs:SBopsem.ECStack) (ECs:LLVMopsem.ECStack) : Prop :=
+  match sbECs, ECs with
+  | sbEC::sbECs', EC::ECs' => 
+      sbEC_simulates_EC_head TD M1 M2 gl mi sbEC EC /\ 
+      sbECs_simulate_ECs_tail TD M1 M2 gl mi sbECs' ECs'
+  | _, _ => False
+  end.
+
+Definition sbState_simulates_State (mi:Values.meminj) (mgb:Values.block) 
+  (sbSt:SBopsem.State) (St:LLVMopsem.State) : Prop :=
+  match (sbSt, St) with
+  | (SBopsem.mkState S1 TD1 Ps1 ECs1 gl1 fs1 M1 MM1,
+     LLVMopsem.mkState S2 TD2 Ps2 ECs2 gl2 fs2 M2) =>
+      let '(los, nts) := TD1 in
+      trans_system S1 = Some S2 /\ 
+      TD1 = TD2 /\ 
+      trans_products nts Ps1 = trans_products nts Ps2 /\ 
+      sbECs_simulate_ECs TD1 M1 M2 gl1 mi ECs1 ECs2 /\
+      gl1 = gl2 /\ 
+      fs1 = fs2 /\ 
+      wf_sb_mi mgb mi M1 M2 /\
+      mem_simulation mi TD1 mgb MM1 M1 M2 
+  end.
+
+Lemma free_allocas_sim : forall TD M1 als1 M2 mi als2 M1' MM mgb lc1 lc2 rm1 rm2 
+    gl ECsc1 ECs2 addrb addre lc,
+  free_allocas TD M1 als1 = Some M1' ->
+  allocas_simulation TD mi lc addrb addre als1 als2 ->
+  mem_simulation mi TD mgb MM M1 M2 ->
+  reg_simulation mi TD gl rm1 rm2 M1 M2 lc1 lc2 ->
+  sbECs_simulate_ECs_tail TD M1 M2 gl mi ECsc1 ECs2 ->
+  wf_sb_mi mgb mi M1 M2 ->
+  exists M2', free_allocas TD M2 als2 = Some M2' /\ 
+    mem_simulation mi TD mgb MM M1' M2' /\
+    reg_simulation mi TD gl rm1 rm2 M1' M2' lc1 lc2 /\
+    sbECs_simulate_ECs_tail TD M1' M2' gl mi ECsc1 ECs2 /\
+    wf_sb_mi mgb mi M1' M2'.
+Admitted.
+
+Definition sb_fnattrs := fnattrs_intro linkage_external visibility_default 
+  callconv_ccc nil nil.
+
+Axiom dstk_spec : forall M, 
+  LLVMopsem.callExternalFunction M dstk_fid nil = Some (None, M).
+
+Axiom dstk_is_found : forall TD M Ps gl lc fs, 
+  LLVMopsem.lookupExFdecViaGV TD M Ps gl lc fs dstk_fn = Some
+    (fdec_intro (fheader_intro sb_fnattrs dstk_typ dstk_fid nil false)).
+
+Definition int2GV n :=
+  (Vint 31 (Int.repr 31 (INTEGER.to_Z n)), AST.Mint 31)::nil.
+
+Axiom stk_ret_sim : forall TD M1 M2 mi MM mgb lc1 lc2 rm1 rm2 gl ECsc1 ECs2 bgv
+    egv,
+  mem_simulation mi TD mgb MM M1 M2 ->
+  reg_simulation mi TD gl rm1 rm2 M1 M2 lc1 lc2 ->
+  sbECs_simulate_ECs_tail TD M1 M2 gl mi ECsc1 ECs2 ->
+  wf_sb_mi mgb mi M1 M2 ->
+  exists M2',  exists M2'',
+    LLVMopsem.callExternalFunction M2 sbase_fid (bgv::int2GV 0%Z::nil) = 
+      Some (None, M2') /\
+    LLVMopsem.callExternalFunction M2' sbound_fid (egv::int2GV 0%Z::nil) = 
+      Some (None, M2'') /\
+    mem_simulation mi TD mgb MM M1 M2'' /\
+    reg_simulation mi TD gl rm1 rm2 M1 M2'' lc1 lc2 /\
+    sbECs_simulate_ECs_tail TD M1 M2'' gl mi ECsc1 ECs2 /\
+    wf_sb_mi mgb mi M1 M2'' /\
+    LLVMopsem.callExternalFunction M2'' gbase_fid [int2GV 0%Z] = 
+      Some (Some bgv, M2'') /\
+    LLVMopsem.callExternalFunction M2'' gbound_fid [int2GV 0%Z] = 
+      Some (Some egv, M2'').
+
+Axiom sbase_is_found : forall TD M Ps gl lc fs, 
+  LLVMopsem.lookupExFdecViaGV TD M Ps gl lc fs sbase_fn = Some
+    (fdec_intro (fheader_intro sb_fnattrs dstk_typ sbase_fid nil false)).
+
+Axiom sbound_is_found : forall TD M Ps gl lc fs, 
+  LLVMopsem.lookupExFdecViaGV TD M Ps gl lc fs sbound_fn = Some
+    (fdec_intro (fheader_intro sb_fnattrs dstk_typ sbound_fid nil false)).
+
+Axiom gbase_is_found : forall TD M Ps gl lc fs, 
+  LLVMopsem.lookupExFdecViaGV TD M Ps gl lc fs gbase_fn = Some
+    (fdec_intro (fheader_intro sb_fnattrs dstk_typ gbase_fid nil false)).
+
+Axiom gbound_is_found : forall TD M Ps gl lc fs, 
+  LLVMopsem.lookupExFdecViaGV TD M Ps gl lc fs gbound_fn = Some
+    (fdec_intro (fheader_intro sb_fnattrs dstk_typ gbound_fid nil false)).
+
+Lemma SBpass_is_correct : forall mi mgb sbSt St sbSt' tr,
+  sbState_simulates_State mi mgb sbSt St ->
+  SBopsem.dsInsn sbSt sbSt' tr -> 
+  exists St', exists mi',
+    LLVMopsem.dsop_star St St' tr /\    
+    sbState_simulates_State mi' mgb sbSt' St' /\
+    Values.inject_incr mi mi'.
+Proof.
+  intros mi mgb sbSt St sbSt' tr Hsim Hsbop.
+  (sb_dsInsn_cases (induction Hsbop) Case).
+Case "dsReturn". Focus.
+  destruct St as [S2 TD2 Ps2 ECs2 gl2 fs2 M2].
+  destruct TD as [los nts].
+  destruct Hsim as [Htsym [Heq1 [Htps [HsimECs [Heq2 [Heq3 [Hwfmi HsimM]]]]]]];
+    subst.
+  destruct ECs2 as [|[F2 B2 cs2 tmn2 lc2 als2] ECs2];
+    try solve [inversion HsimECs].
+  simpl in HsimECs.
+  destruct HsimECs as [HsimEC HsimECs].
+  destruct ECs2 as [|[F2' B2' cs2' tmn2' lc2' als2'] ECs2];
+    try solve [inversion HsimECs].
+  destruct HsimECs as [HsimEC' HsimECs].
+  destruct F as [fh1 bs1].
+  destruct F2 as [fh2 bs2].
+  destruct HsimEC as [Htfdef [Heq0 [Hnth [Heqb1 [Heqb2 [ex_ids [rm2 
+    [addrb [ex_ids1 [addre [ex_ids2 [ex_ids3 [ex_ids4 [cs22 [cs23 
+    [Hgenmeta [Hrsim [Hmk1 [Hmk2 [Hals 
+    [Hinc [Htcmds [Httmn Heq1]]]]]]]]]]]]]]]]]]]]]]]; subst.
+  destruct F' as [fh1' bs1'].
+  destruct F2' as [fh2' bs2'].
+  destruct c'; try solve [inversion HsimEC'].  
+  destruct HsimEC' as [Htfdef' [Heq0' [Hnth' [Heqb1' [Heqb2'
+    [ex_ids' [rm2' [addrb' [ex_ids1' [addre' [ex_ids2' 
+    [ex_ids3' [ex_ids4' [cs22' [cs23' [cs24' 
+    [Hgenmeta' [Hrsim' [Hmk1' [Hmk2' [Hals' 
+    [Hinc' [Hcall' [Htcmds' [Httmn' Heq1']]]]]]]]]]]]]]]]]]]]]]]]]; subst.
+  inv Htcmds.
+  simpl in H1.
+  unfold call_suffix in Hcall'.
+  unfold SBopsem.returnUpdateLocals in H1.
+  remember (SBopsem.returnResult (los, nts) Mem' RetTy Result lc rm gl2) as Ret.
+  destruct Ret as [[gr md]|]; try solve [inv H1].
+  unfold SBopsem.returnResult in HeqRet.
+  remember (getOperandValue (los, nts) Mem' Result lc gl2) as ogr.
+  destruct ogr as [ogr|]; try solve [inv HeqRet].
+  destruct n.
+  SCase "nret = true".
+    inv Hcall'.
+    inv H1.
+    simpl in Httmn.
+    destruct (isPointerTypB RetTy).
+    SSCase "rt is ptr". Focus.
+      remember (SBopsem.get_reg_metadata (los, nts) Mem' gl2 rm Result) as oRmd.
+      destruct oRmd as [[bgv1 egv1]|]; inv HeqRet.
+      assert (exists bv2, exists ev2, exists bgv2, exists egv2,
+        get_reg_metadata rm2 Result = Some (bv2, ev2) /\
+        getOperandValue (los,nts) M2 bv2 lc2 gl2 = Some bgv2 /\
+        getOperandValue (los,nts) M2 ev2 lc2 gl2 = Some egv2 /\
+        gv_inject mi bgv1 bgv2 /\
+        gv_inject mi egv1 egv2) as J.
+        clear - HeqoRmd Hrsim. 
+        destruct Hrsim as [_ Hrsim].
+        apply Hrsim; auto.
+          admit. (* const2GV *)
+      destruct J as [bv2 [ev2 [bgv2 [egv2 [Hgetrmd [Hgetbgv2 [Hgetegv2 [Hinj1 
+        Hinj2]]]]]]]]. rewrite Hgetrmd in Httmn. inv Httmn.
+Admitted.
+(*
+      destruct (@stk_ret_sim (los,nts) Mem M2 mi MM mgb lc'' lc2' rm'' rm2'
+        gl2 EC ECs2 bv null) as [M2' [M2'' [Hsbase [Hsbound [Hmsim3 [Hrsim3
+        [HsimECs3 [Hwfmi3 [Hgbase Hgbound]]]]]]]]]; auto.
+      eapply free_allocas_sim with (rm1:=rm'')(rm2:=rm2')(lc1:=lc'')(lc2:=lc2') 
+        in HsimECs3; eauto.
+      destruct HsimECs3 as [M2''' [Hfree2' [Hmsim2' [Hrsim2' [HsimECs2' Hwfmi2']]
+        ]]].
+      exists (LLVMopsem.mkState S2 (los, nts) Ps2
+        ((LLVMopsem.mkEC (fdef_intro fh2' bs2') B2'
+            (cs23' ++ cs24') tmn2' lc2' als2'):: ECs2)
+        gl2 fs2 M2''').
+      exists mi.
+      split.
+      SSSCase "dsop_star".
+        rewrite <- (@trace_app_nil__eq__trace trace_nil).
+        apply LLVMopsem.dsop_star_cons with (state2:=
+          (LLVMopsem.mkState S2 (los, nts) Ps2
+            ((LLVMopsem.mkEC (fdef_intro fh2 bs2) B2
+              ((insn_call fake_id true attrs sbound_typ sbound_fn 
+                  ((p8, vnullp8)::(i32, vint0) :: nil))::nil)
+              (insn_return rid RetTy Result) lc2 als2)::
+             (LLVMopsem.mkEC (fdef_intro fh2' bs2') B2'
+              ((insn_call i0 true c t (wrap_call v) p)::
+               (insn_call fake_id true attrs dstk_typ dstk_fn nil)::
+              (cs23' ++ cs24'))
+              tmn2' lc2' als2'):: ECs2)
+            gl2 fs2 M2')).
+          eapply LLVMopsem.dsExCall with (fid:=sbase_fid)
+            (gvs:=(null :: int2GV 0 :: nil))(oresult:=None); eauto.
+            eapply sbase_is_found; eauto.
+        rewrite <- (@trace_app_nil__eq__trace trace_nil).
+        apply LLVMopsem.dsop_star_cons with (state2:=
+          (LLVMopsem.mkState S2 (los, nts) Ps2
+            ((LLVMopsem.mkEC (fdef_intro fh2 bs2) B2 nil
+              (insn_return rid RetTy Result) lc2 als2)::
+             (LLVMopsem.mkEC (fdef_intro fh2' bs2') B2'
+              ((insn_call i0 true c t (wrap_call v) p)::
+               (insn_call fake_id true attrs dstk_typ dstk_fn nil)::
+              (cs23' ++ cs24'))
+              tmn2' lc2' als2'):: ECs2)
+            gl2 fs2 M2'')).
+          eapply LLVMopsem.dsExCall with (fid:=sbound_fid)
+            (gvs:=(null :: int2GV 0 :: nil))(oresult:=None); eauto.
+            eapply sbound_is_found; eauto.
+        rewrite <- (@trace_app_nil__eq__trace trace_nil).
+        apply LLVMopsem.dsop_star_cons with (state2:=
+          (LLVMopsem.mkState S2 (los, nts) Ps2
+            ((LLVMopsem.mkEC (fdef_intro fh2' bs2') B2'
+              ((insn_call fake_id true attrs dstk_typ dstk_fn nil)::
+              (cs23' ++ cs24'))
+              tmn2' lc2' als2'):: ECs2)
+            gl2 fs2 M2''')).
+          eapply LLVMopsem.dsReturn; eauto.
+        rewrite <- (@trace_app_nil__eq__trace trace_nil).
+        apply LLVMopsem.dsop_star_cons with (state2:=
+          (LLVMopsem.mkState S2 (los, nts) Ps2
+            ((LLVMopsem.mkEC (fdef_intro fh2' bs2') B2'
+              (cs23' ++ cs24')
+              tmn2' lc2' als2'):: ECs2)
+            gl2 fs2 M2''')); auto.
+          eapply LLVMopsem.dsExCall; simpl; eauto.
+            eapply dstk_is_found; eauto.
+            eapply dstk_spec; eauto.
+
+      split; auto using inject_incr_refl.
+      SSSCase "sim".
+      repeat (split; auto).
+          destruct Heqb1' as [l1' [ps1' [cs11' Heqb1']]]; subst.
+          exists l1'. exists ps1'. 
+          exists (cs11' ++ [insn_call i0 true c t v p]). 
+          simpl_env. auto.
+
+          destruct Heqb2' as [l2' [ps2' [cs21' Heqb2']]]; subst.
+          exists l2'. exists ps2'. exists (cs21' ++
+              [insn_call i0 true c t (wrap_call v) p] ++
+              [insn_call fake_id true attrs dstk_typ dstk_fn nil]). 
+          simpl_env. auto.
+ 
+          exists ex_ids'. exists rm2'.
+          exists addrb'. exists ex_ids1'. exists addre'. exists ex_ids2'. 
+          exists ex_ids3'. exists ex_ids4'. exists cs23'. exists cs24'.
+          repeat (split; auto).
+
+
+    SSCase "rt isnt ptr".
+      inv Httmn.
+      destruct (@stk_ret_sim (los,nts) Mem M2 mi MM mgb lc'' lc2' rm'' rm2'
+        gl2 EC ECs2 null null) as [M2' [M2'' [Hsbase [Hsbound [Hmsim3 [Hrsim3
+        [HsimECs3 [Hwfmi3 [Hgbase Hgbound]]]]]]]]]; auto.
+      eapply free_allocas_sim with (rm1:=rm'')(rm2:=rm2')(lc1:=lc'')(lc2:=lc2') 
+        in HsimECs3; eauto.
+      destruct HsimECs3 as [M2''' [Hfree2' [Hmsim2' [Hrsim2' [HsimECs2' Hwfmi2']]
+        ]]].
+      exists (LLVMopsem.mkState S2 (los, nts) Ps2
+        ((LLVMopsem.mkEC (fdef_intro fh2' bs2') B2'
+            (cs23' ++ cs24') tmn2' lc2' als2'):: ECs2)
+        gl2 fs2 M2''').
+      exists mi.
+      split.
+      SSSCase "dsop_star".
+        rewrite <- (@trace_app_nil__eq__trace trace_nil).
+        apply LLVMopsem.dsop_star_cons with (state2:=
+          (LLVMopsem.mkState S2 (los, nts) Ps2
+            ((LLVMopsem.mkEC (fdef_intro fh2 bs2) B2
+              ((insn_call fake_id true attrs sbound_typ sbound_fn 
+                  ((p8, vnullp8)::(i32, vint0) :: nil))::nil)
+              (insn_return rid RetTy Result) lc2 als2)::
+             (LLVMopsem.mkEC (fdef_intro fh2' bs2') B2'
+              ((insn_call i0 true c t (wrap_call v) p)::
+               (insn_call fake_id true attrs dstk_typ dstk_fn nil)::
+              (cs23' ++ cs24'))
+              tmn2' lc2' als2'):: ECs2)
+            gl2 fs2 M2')).
+          eapply LLVMopsem.dsExCall with (fid:=sbase_fid)
+            (gvs:=(null :: int2GV 0 :: nil))(oresult:=None); eauto.
+            eapply sbase_is_found; eauto.
+        rewrite <- (@trace_app_nil__eq__trace trace_nil).
+        apply LLVMopsem.dsop_star_cons with (state2:=
+          (LLVMopsem.mkState S2 (los, nts) Ps2
+            ((LLVMopsem.mkEC (fdef_intro fh2 bs2) B2 nil
+              (insn_return rid RetTy Result) lc2 als2)::
+             (LLVMopsem.mkEC (fdef_intro fh2' bs2') B2'
+              ((insn_call i0 true c t (wrap_call v) p)::
+               (insn_call fake_id true attrs dstk_typ dstk_fn nil)::
+              (cs23' ++ cs24'))
+              tmn2' lc2' als2'):: ECs2)
+            gl2 fs2 M2'')).
+          eapply LLVMopsem.dsExCall with (fid:=sbound_fid)
+            (gvs:=(null :: int2GV 0 :: nil))(oresult:=None); eauto.
+            eapply sbound_is_found; eauto.
+        rewrite <- (@trace_app_nil__eq__trace trace_nil).
+        apply LLVMopsem.dsop_star_cons with (state2:=
+          (LLVMopsem.mkState S2 (los, nts) Ps2
+            ((LLVMopsem.mkEC (fdef_intro fh2' bs2') B2'
+              ((insn_call fake_id true attrs dstk_typ dstk_fn nil)::
+              (cs23' ++ cs24'))
+              tmn2' lc2' als2'):: ECs2)
+            gl2 fs2 M2''')).
+          eapply LLVMopsem.dsReturn; eauto.
+        rewrite <- (@trace_app_nil__eq__trace trace_nil).
+        apply LLVMopsem.dsop_star_cons with (state2:=
+          (LLVMopsem.mkState S2 (los, nts) Ps2
+            ((LLVMopsem.mkEC (fdef_intro fh2' bs2') B2'
+              (cs23' ++ cs24')
+              tmn2' lc2' als2'):: ECs2)
+            gl2 fs2 M2''')); auto.
+          eapply LLVMopsem.dsExCall; simpl; eauto.
+            eapply dstk_is_found; eauto.
+            eapply dstk_spec; eauto.
+
+      split; auto using inject_incr_refl.
+      SSSCase "sim".
+      repeat (split; auto).
+          destruct Heqb1' as [l1' [ps1' [cs11' Heqb1']]]; subst.
+          exists l1'. exists ps1'. 
+          exists (cs11' ++ [insn_call i0 true c t v p]). 
+          simpl_env. auto.
+
+          destruct Heqb2' as [l2' [ps2' [cs21' Heqb2']]]; subst.
+          exists l2'. exists ps2'. exists (cs21' ++
+              [insn_call i0 true c t (wrap_call v) p] ++
+              [insn_call fake_id true attrs dstk_typ dstk_fn nil]). 
+          simpl_env. auto.
+ 
+          exists ex_ids'. exists rm2'.
+          exists addrb'. exists ex_ids1'. exists addre'. exists ex_ids2'. 
+          exists ex_ids3'. exists ex_ids4'. exists cs23'. exists cs24'.
+          repeat (split; auto).
+
+  SCase "nret = false".
+    remember (getOperandValue (los, nts) Mem' Result lc gl2) as R.
+    destruct R; try solve [inv H1].
+    destruct (SBopsem.isReturnPointerTypB t); simpl in Hcall'.
+    SSCase "ct is ptr".
+      simpl in Httmn.
+      destruct (isPointerTypB RetTy).
+    SSSCase "rt is ptr".
+      destruct (get_reg_metadata rm2 Result) as [[bv ev]|]; inv Httmn.
+
+
+
+    inv H1.
+    inv Hcall'.
+
+    SSCase "rt isnt ptr".
+      inv Httmn.
+      destruct (@stk_ret_sim (los,nts) Mem M2 mi MM mgb lc'' lc2' rm'' rm2'
+        gl2 EC ECs2 null null) as [M2' [M2'' [Hsbase [Hsbound [Hmsim3 [Hrsim3
+        [HsimECs3 [Hwfmi3 [Hgbase Hgbound]]]]]]]]]; auto.
+      eapply free_allocas_sim with (rm1:=rm'')(rm2:=rm2')(lc1:=lc'')(lc2:=lc2') 
+        in HsimECs3; eauto.
+      destruct HsimECs3 as [M2''' [Hfree2' [Hmsim2' [Hrsim2' [HsimECs2' Hwfmi2']]
+        ]]].
+      exists (LLVMopsem.mkState S2 (los, nts) Ps2
+        ((LLVMopsem.mkEC (fdef_intro fh2' bs2') B2'
+            (cs23' ++ cs24') tmn2' lc2' als2'):: ECs2)
+        gl2 fs2 M2''').
+      exists mi.
+      split.
+      SSSCase "dsop_star".
+        rewrite <- (@trace_app_nil__eq__trace trace_nil).
+        apply LLVMopsem.dsop_star_cons with (state2:=
+          (LLVMopsem.mkState S2 (los, nts) Ps2
+            ((LLVMopsem.mkEC (fdef_intro fh2 bs2) B2
+              ((insn_call fake_id true attrs sbound_typ sbound_fn 
+                  ((p8, vnullp8)::(i32, vint0) :: nil))::nil)
+              (insn_return rid RetTy Result) lc2 als2)::
+             (LLVMopsem.mkEC (fdef_intro fh2' bs2') B2'
+              ((insn_call i0 true c t (wrap_call v) p)::
+               (insn_call fake_id true attrs dstk_typ dstk_fn nil)::
+              (cs23' ++ cs24'))
+              tmn2' lc2' als2'):: ECs2)
+            gl2 fs2 M2')).
+          eapply LLVMopsem.dsExCall with (fid:=sbase_fid)
+            (gvs:=(null :: int2GV 0 :: nil))(oresult:=None); eauto.
+            eapply sbase_is_found; eauto.
+        rewrite <- (@trace_app_nil__eq__trace trace_nil).
+        apply LLVMopsem.dsop_star_cons with (state2:=
+          (LLVMopsem.mkState S2 (los, nts) Ps2
+            ((LLVMopsem.mkEC (fdef_intro fh2 bs2) B2 nil
+              (insn_return rid RetTy Result) lc2 als2)::
+             (LLVMopsem.mkEC (fdef_intro fh2' bs2') B2'
+              ((insn_call i0 true c t (wrap_call v) p)::
+               (insn_call fake_id true attrs dstk_typ dstk_fn nil)::
+              (cs23' ++ cs24'))
+              tmn2' lc2' als2'):: ECs2)
+            gl2 fs2 M2'')).
+          eapply LLVMopsem.dsExCall with (fid:=sbound_fid)
+            (gvs:=(null :: int2GV 0 :: nil))(oresult:=None); eauto.
+            eapply sbound_is_found; eauto.
+        rewrite <- (@trace_app_nil__eq__trace trace_nil).
+        apply LLVMopsem.dsop_star_cons with (state2:=
+          (LLVMopsem.mkState S2 (los, nts) Ps2
+            ((LLVMopsem.mkEC (fdef_intro fh2' bs2') B2'
+              ((insn_call fake_id true attrs dstk_typ dstk_fn nil)::
+              (cs23' ++ cs24'))
+              tmn2' lc2' als2'):: ECs2)
+            gl2 fs2 M2''')).
+          eapply LLVMopsem.dsReturn; eauto.
+        rewrite <- (@trace_app_nil__eq__trace trace_nil).
+        apply LLVMopsem.dsop_star_cons with (state2:=
+          (LLVMopsem.mkState S2 (los, nts) Ps2
+            ((LLVMopsem.mkEC (fdef_intro fh2' bs2') B2'
+              (cs23' ++ cs24')
+              tmn2' lc2' als2'):: ECs2)
+            gl2 fs2 M2''')); auto.
+          eapply LLVMopsem.dsExCall; simpl; eauto.
+            eapply dstk_is_found; eauto.
+            eapply dstk_spec; eauto.
+
+      split; auto using inject_incr_refl.
+      SSSCase "sim".
+      repeat (split; auto).
+          destruct Heqb1' as [l1' [ps1' [cs11' Heqb1']]]; subst.
+          exists l1'. exists ps1'. 
+          exists (cs11' ++ [insn_call i0 true c t v p]). 
+          simpl_env. auto.
+
+          destruct Heqb2' as [l2' [ps2' [cs21' Heqb2']]]; subst.
+          exists l2'. exists ps2'. exists (cs21' ++
+              [insn_call i0 true c t (wrap_call v) p] ++
+              [insn_call fake_id true attrs dstk_typ dstk_fn nil]). 
+          simpl_env. auto.
+ 
+          exists ex_ids'. exists rm2'.
+          exists addrb'. exists ex_ids1'. exists addre'. exists ex_ids2'. 
+          exists ex_ids3'. exists ex_ids4'. exists cs23'. exists cs24'.
+          repeat (split; auto).
+*)
+
+(*****************************)
+(*
+*** Local Variables: ***
+*** coq-prog-name: "coqtop" ***
+*** coq-prog-args: ("-emacs-U" "-I" "~/SVN/sol/vol/src/ssa/monads" "-I" "~/SVN/sol/vol/src/ssa/ott" "-I" "~/SVN/sol/vol/src/ssa/compcert" "-I" "~/SVN/sol/theory/metatheory_8.3" "-I" "~/SVN/sol/vol/src/TV") ***
+*** End: ***
+ *)
